refactor

paxos/synod.dfy
@@ -8,45 +8,73 @@ import opened Agents
 import opened Types
 
 
+datatype Constants = Constants(f:nat, ldr_ids:seq<Id>, acc_ids:seq<Id>) {
+    predicate WF() {
+        && f >= 1
+        && |ldr_ids| >= 1
+        && |acc_ids| == 2*f+1
+        && ValidTypes()
+        && UniqueIds()
+    }
+
+    predicate ValidLdrIdx(i:int) {
+        0<=i<|ldr_ids|
+    }
+
+    predicate ValidAccIdx(i:int) {
+        0<=i<|acc_ids|
+    }
+
+    predicate ValidTypes() {
+        && (forall l | l in ldr_ids :: l.agt.Ldr?)
+        && (forall l | l in acc_ids :: l.agt.Acc?)
+    }
+
+    predicate UniqueIds() {
+        && (forall i:nat, j:nat | ValidLdrIdx(i) && ValidLdrIdx(j) && ldr_ids[i]==ldr_ids[j] :: i == j)
+        && (forall i:nat, j:nat | ValidAccIdx(i) && ValidAccIdx(j) && acc_ids[i]==acc_ids[j] :: i == j)
+    }
+}
+
 datatype DistrSys = DistrSys(
     network: Environment,
     leaders: seq<Leader>,
     acceptors: seq<Acceptor>
-)
+) {
+    predicate WF(c: Constants)
+        requires c.WF()
+    {
+        && |leaders| == |c.ldr_ids|
+        && |acceptors| == |c.acc_ids|
+        && (forall i | c.ValidLdrIdx(i) :: leaders[i].consts.id == c.ldr_ids[i])
+        && (forall i | c.ValidAccIdx(i) :: acceptors[i].consts.id == c.acc_ids[i])
+    }
+}
 
 
 /*****************************************************************************************
 *                                        DS Init                                         *
 *****************************************************************************************/
-predicate Init(s:DistrSys, f:nat, l:nat, accConf:seq<Id>) 
+predicate Init(c:Constants, s:DistrSys) 
 {
-    && ValidConf(f, l, accConf)
+    && c.WF()
     && EnvironmentInit(s.network)
-    && |s.leaders| == l
-    && (forall i | 0 <= i < l :: LeaderInit(s.leaders[i], Id(Ldr, i), accConf, f, V(i)))
-    && |s.acceptors| == 2*f+1
-    && (forall i | 0 <= i < 2*f+1 :: AcceptorInit(s.acceptors[i], accConf[i]))
+    && |s.leaders| == |c.ldr_ids|
+    && |s.acceptors| == |c.acc_ids|
+    && (forall i | c.ValidLdrIdx(i) :: LeaderInit(s.leaders[i], c.ldr_ids[i], c.acc_ids, c.f, V(i)))
+    && (forall i | c.ValidAccIdx(i) :: AcceptorInit(s.acceptors[i], c.acc_ids[i]))
 }
-
-predicate ValidConf(f:nat, l:nat, accConf:seq<Id>) {
-    && f >= 1
-    && l >= 1
-    && |accConf| == 2*f+1
-    && (forall i | 0 <= i < |accConf| :: accConf[i] == Id(Acc, i))
-}
-
-// predicate AccConfUnique(accConf:seq<Id>) {
-//     forall i,j | 0 <= i < |accConf| && 0 <= j < |accConf| 
-//     :: accConf[i].idx == accConf[j].idx ==> i == j
-// }
 
 
 /*****************************************************************************************
 *                                        DS Next                                         *
 *****************************************************************************************/
 
-predicate Next(s:DistrSys, s':DistrSys) {
-    exists src, recvIos, sendIos :: PaxosNextOneAgent(s, s', src, recvIos, sendIos)
+predicate Next(c:Constants, s:DistrSys, s':DistrSys) {
+    && c.WF()
+    && s.WF(c)
+    && s'.WF(c)
+    && exists src, recvIos, sendIos :: PaxosNextOneAgent(s, s', src, recvIos, sendIos)
 }
 
 
